@prefix xsd: <http://www.w3.org/2001/XMLSchema#>.
@prefix rdf: <http://www.w3.org/1999/02/22-rdf-syntax-ns#>.
@prefix rdfs: <http://www.w3.org/2000/01/rdf-schema#>.
@prefix owl: <http://www.w3.org/2002/07/owl#>.
@prefix skos: <http://www.w3.org/2004/02/skos/core#>.
@prefix skoslex: <http://bp4mc2.org/def/skos-lex/>.
@prefix thes: <http://purl.org/iso25964/skos-thes#>.

skoslex:Act a owl:Class;
	rdfs:subClassOf skos:Concept;
	rdfs:label "Act"@en;
	rdfs:label "Handeling"@nl;
	rdfs:comment "Een handeling is een concept dat verwijst naar een afgeronde hoeveelheid werk met een overdraagbaar resultaat";
	rdfs:comment "An act is a concept that refers to a distinct piece of work that produces some result";
.

skoslex:Norm a owl:Class;
	rdfs:subClassOf skos:Concept;
	rdfs:label "Norm"@en;
	rdfs:label "Norm"@nl;
	rdfs:comment "Een norm is een concept dat regels stelt waaraan een handeling moet voldoen";
	rdfs:comment "A norm is a concept that refers to the conditions an act must meet";
.

skoslex:Actor a owl:Class;
	rdfs:subClassOf skos:Concept;
	rdfs:label "Actor"@en;
	rdfs:label "Actor"@nl;
	rdfs:comment "An actor is someone who performs an act";
.

skoslex:Agent a owl:Class;
	rdfs:subClassOf skoslex:Actor;
	rdfs:label "Agent"@en;
	rdfs:label "Agent"@nl;
	rdfs:comment "An agent is someone who supports an act. The agent is not realy part of the act, but is needed for the act to take place."
.

skoslex:Object a owl:Class;
	rdfs:subClassOf skos:Concept;
	rdfs:label "Object"@en;
	rdfs:label "Object"@nl;
	rdfs:comment "An object that is applied with an act";
.

skoslex:performedBy a owl:ObjectProperty;
	rdfs:subPropertyOf skos:semanticRelation;
	rdfs:domain skoslex:Act;
	rdfs:range skoslex:Actor;
.
skoslex:supportedBy a owl:ObjectProperty;
	rdfs:subPropertyOf skos:semanticRelation;
	rdfs:domain skoslex:Act;
	rdfs:range skoslex:Agent;
.

skoslex:affects a owl:ObjectProperty;
	rdfs:subPropertyOf skos:semanticRelation;
	rdfs:comment "States the act that is affected by the norm. The act should meet the conditions of the norm";
.

skoslex:appliedWith a owl:ObjectProperty;
	rdfs:subPropertyOf skos:semanticRelation;
	rdfs:domain skoslex:Act;
	rdfs:range: skoslex:Object;
	rdfs:comment "States the relationship between an act and the applied object";
.

skoslex:refersTo a owl:ObjectProperty;
	rdfs:subPropertyOf skos:semanticRelation;
	rdfs:domain skoslex:Norm;
	rdfs:range skoslex:Act;
	rdfs:comment "States that a norm refers to some act. The norm doesn't set conditions for this act, but the act is in some way part of the condition itself (for example: the act should be performed as a precondition for another act.";
.
